

Bivariate Normal

Snehal M. Shekatkar

1 Derivation of the density formula

We will generalize the notion of a univariate normal distribution to two dimensions by demanding that the contours of constant density are ellipses. Consider a general equation of ellipse:

$$Ax_1^2 + 2Bx_1x_2 + Cx_2^2 = k$$

The LHS can be rewritten in a matrix form as:

$$\mathbf{x}^T \mathbf{M} \mathbf{x} = \begin{bmatrix} x_1 & x_2 \end{bmatrix} \begin{bmatrix} A & B \\ B & C \end{bmatrix} \begin{bmatrix} x_1 \\ x_2 \end{bmatrix}$$

We will demand that the density should drop as exponential of this:

$$p(\mathbf{X}) = \frac{1}{Z} e^{-\mathbf{x}^T \mathbf{M} \mathbf{x}}$$

where $1/Z$ is the constant of proportionality to be determined. For the point \mathbf{x} on a given ellipse, the quantity $\mathbf{x}^T \mathbf{M} \mathbf{x}$ is called *Mahalanobis distance*. Later we will see that for appropriate choice of matrix M , this represents the distance of a point on a circle from its center. Since we don't want it to be negative, we see that M must be a *positive-definite matrix*.

Throughout the discussion of the bivariate normal, we will use the following Gaussian integral formula:

$$\int_0^\infty x^m e^{-\beta x^n} dx = \frac{1}{n} \frac{\Gamma(\frac{m+1}{n})}{\beta^{\frac{m+1}{n}}} \quad (1)$$

where $\Gamma(n+1) = n\Gamma(n)$, and $\Gamma(\frac{1}{2}) = \sqrt{\pi}$.

Clearly,

$$\begin{aligned} Z &= \int_{x_1=-\infty}^{\infty} \int_{x_2=-\infty}^{\infty} \exp(-Ax_1^2 - 2Bx_1x_2 - Cx_2^2) dx_2 dx_1 \\ &= \int_{x_1=-\infty}^{\infty} e^{-Ax_1^2} \left[\int_{x_2=-\infty}^{\infty} e^{-2Bx_1x_2 - Cx_2^2} dx_2 \right] dx_1 \end{aligned} \quad (2)$$

Let us first consider the inner integral:

$$I_{x_2} = \int_{x_2=-\infty}^{\infty} e^{-2Bx_1x_2 - Cx_2^2} dx_2 \quad (3)$$

To compute this integral, we can complete the square in x_2 :

$$\begin{aligned} 2Bx_1x_2 + Cx_2^2 &= C \left(x_2^2 + 2\frac{B}{C}x_1x_2 \right) = C \left(x_2 + \frac{B}{C}x_1 \right)^2 - \frac{B^2}{C}x_1^2 \\ I_{x_2} &= e^{\frac{B^2}{C}x_1^2} \int_{x_2=-\infty}^{\infty} \exp \left[-C \left(x_2 + \frac{B}{C}x_1 \right)^2 \right] dx_2 \end{aligned} \quad (4)$$

To compute the integral, we can substitute $x'_2 = x_2 + \frac{B}{C}x_1$. Hence:

$$\begin{aligned}
I_{x_2} &= e^{\frac{B^2}{C}x_1^2} \int_{x'_2=-\infty}^{\infty} e^{-Cx_2'^2} dx'_2 = e^{\frac{B^2}{C}x_1^2} \times 2 \int_{x'_2=0}^{\infty} e^{-Cx_2'^2} dx'_2 \\
&= e^{\frac{B^2}{C}x_1^2} \times 2 \times \frac{1}{2} \frac{\Gamma(1/2)}{\sqrt{C}} \\
&= \sqrt{\frac{\pi}{C}} e^{\frac{B^2}{C}x_1^2}
\end{aligned} \tag{5}$$

Putting this in 2, we get:

$$\begin{aligned}
Z &= \int_{x_1=-\infty}^{\infty} e^{-Ax_1^2} \sqrt{\frac{\pi}{C}} e^{\frac{B^2}{C}x_1^2} dx_1 \\
&= \sqrt{\frac{\pi}{C}} \int_{x_1=-\infty}^{\infty} e^{-\left(A - \frac{B^2}{C}\right)x_1^2} dx_1 \\
&= \sqrt{\frac{\pi}{C}} \times 2 \times \int_{x_1=0}^{\infty} e^{-\left(A - \frac{B^2}{C}\right)x_1^2} dx_1 \\
&= \sqrt{\frac{\pi}{C}} \times 2 \times \frac{1}{2} \frac{\Gamma(1/2)}{\left(A - \frac{B^2}{C}\right)^{1/2}}
\end{aligned} \tag{6}$$

$$\boxed{\therefore Z = \frac{\pi}{\sqrt{AC - B^2}}} \tag{7}$$

Let us now compute the marginal distribution of x_1 by integrating over x_2 :

$$\begin{aligned}
p_{X_1}(x) &= \int_{x_2=-\infty}^{\infty} \frac{1}{Z} e^{-(Ax_1^2 + 2Bx_1x_2 + Cx_2^2)} dx_2 \\
&= \frac{1}{Z} e^{-Ax_1^2} \int_{x_2=-\infty}^{\infty} e^{-(2Bx_1x_2 + Cx_2^2)} dx_2 = \frac{1}{Z} e^{-Ax_1^2} I_{x_2} \\
&= \frac{\sqrt{AC - B^2}}{\pi} e^{-Ax_1^2} \sqrt{\frac{\pi}{C}} e^{\frac{B^2}{C}x_1^2} \\
&= \sqrt{\frac{AC - B^2}{\pi C}} e^{-\left(A - \frac{B^2}{C}\right)x_1^2}
\end{aligned} \tag{8}$$

$$\boxed{\therefore p_{X_1}(x) = \sqrt{\frac{AC - B^2}{\pi C}} \exp \left[- \left(\frac{AC - B^2}{C} \right) x_1^2 \right]} \tag{9}$$

But this is just the univariate Gaussian distribution with mean zero! Comparing the terms with the variance terms in the univariate Gaussian distribution formula, we see that:

$$\sigma_{x_1}^2 = \frac{C}{2(AC - B^2)} \tag{10}$$

Similarly, marginalizing over x_1 , we see that the distribution of x_2 is also Gaussian:

$$\boxed{\therefore p_{X_2}(x) = \sqrt{\frac{AC - B^2}{\pi A}} \exp \left[- \left(\frac{AC - B^2}{A} \right) x_1^2 \right]} \tag{11}$$

and hence:

$$\sigma_{x_2}^2 = \frac{A}{2(AC - B^2)} \quad (12)$$

Since the means of X_1 and X_2 are zero, we can also compute the correlation between X_1 and X_2 as:

$$\begin{aligned} \text{Cov}(X_1, X_2) &= \mathbb{E}[X_1 X_2] = \frac{1}{Z} \int_{-\infty}^{\infty} \int_{-\infty}^{\infty} x_1 x_2 \exp(-Ax_1^2 - 2Bx_1 x_2 - Cx_2^2) dx_2 dx_1 \\ &= \frac{1}{Z} \int_{-\infty}^{\infty} x_1 e^{-Ax_1^2} \left[\int_{-\infty}^{\infty} x_2 e^{-2Bx_1 x_2 - Cx_2^2} dx_2 \right] dx_1 \end{aligned} \quad (13)$$

Now consider the inner integral:

$$I_{xx_2} = \int_{-\infty}^{\infty} x_2 e^{-2Bx_1 x_2 - Cx_2^2} dx_2 \quad (14)$$

Proceeding as before,

$$\begin{aligned} I_{xx_2} &= e^{\frac{B^2}{C}x_1^2} \int_{x_2=-\infty}^{\infty} x_2 \exp \left[-C \left(x_2 + \frac{B}{C}x_1 \right)^2 \right] dx_2 \\ &= e^{\frac{B^2}{C}x_1^2} \int_{x_2=-\infty}^{\infty} \left(x_2 - \frac{B}{C}x_1 \right) e^{-Cx_2^2} dx_2 \\ &= e^{\frac{B^2}{C}x_1^2} \int_{-\infty}^{\infty} x_2 e^{-Cx_2^2} dx_2 - e^{\frac{B^2}{C}x_1^2} \frac{B}{C}x_1 \int_{-\infty}^{\infty} e^{-Cx_2^2} dx_2 \end{aligned} \quad (15)$$

The first of these integrals, being an odd-integral, is zero. Thus,

$$\begin{aligned} I_{xx_2} &= -e^{\frac{B^2}{C}x_1^2} \frac{B}{C}x_1 \int_{-\infty}^{\infty} e^{-Cx_2^2} dx_2 = -e^{\frac{B^2}{C}x_1^2} \frac{B}{C}x_1 \times 2 \times \int_0^{\infty} e^{-Cx_2^2} dx_2 \\ &= -e^{\frac{B^2}{C}x_1^2} \frac{B}{C}x_1 \times 2 \times \frac{1}{2} \frac{\Gamma(1/2)}{C^{1/2}} \\ &= -x_1 e^{\frac{B^2}{C}x_1^2} \frac{B\sqrt{\pi}}{C^{3/2}} \end{aligned} \quad (16)$$

Putting this in 13, we get:

$$\begin{aligned}
\text{Cov}(X_1, X_2) &= \frac{1}{Z} \int_{-\infty}^{\infty} x_1 e^{-Ax_1^2} \left(-x_1 e^{\frac{B^2}{C}x_1^2} \frac{B\sqrt{\pi}}{C^{3/2}} \right) dx_1 \\
&= \frac{-1}{Z} \frac{B\sqrt{\pi}}{C^{3/2}} \int_{-\infty}^{\infty} x_1^2 e^{-Ax_1^2} \left(x_1 e^{\frac{B^2}{C}x_1^2} \right) dx_1 \\
&= \frac{-1}{Z} \frac{B\sqrt{\pi}}{C^{3/2}} \int_{-\infty}^{\infty} x_1^2 e^{-\left(A - \frac{B^2}{C}\right)x_1^2} dx_1 \\
&= \frac{-1}{Z} \frac{B\sqrt{\pi}}{C^{3/2}} \times 2 \times \int_0^{\infty} x_1^2 e^{-\left(A - \frac{B^2}{C}\right)x_1^2} dx_1 \\
&= \frac{-1}{Z} \frac{B\sqrt{\pi}}{C^{3/2}} \times 2 \times \frac{1}{2} \frac{\Gamma(\frac{3}{2})}{\left(A - \frac{B^2}{C}\right)^{3/2}} \\
&= \frac{-1}{Z} \frac{B\sqrt{\pi}}{C^{3/2}} \frac{(\sqrt{\pi}/2)C^{3/2}}{(AC - B^2)^{3/2}} \\
&= \frac{-B\pi}{2Z(AC - B^2)^{3/2}}
\end{aligned} \tag{17}$$

Using the value of Z from (7), we get:

$$\text{Cov}(X_1, X_2) = \frac{\sqrt{AC - B^2}}{2\pi} \times \frac{-B\pi}{(AC - B^2)^{3/2}} \tag{18}$$

$$\boxed{\therefore \text{Cov}(X_1, X_2) = \frac{-B}{2(AC - B^2)}} \tag{19}$$

Hence the full covariance matrix is:

$$\Sigma = \begin{bmatrix} \frac{C}{2(AC - B^2)} & \frac{-B}{2(AC - B^2)} \\ \frac{-B}{2(AC - B^2)} & \frac{A}{2(AC - B^2)} \end{bmatrix} = \frac{1}{2} M^{-1} \tag{20}$$

$$\therefore M = \frac{1}{2} \Sigma^{-1} \tag{21}$$

Also, then from Eq(7), we have:

$$Z = \frac{\pi}{\sqrt{AC - B^2}} = \frac{\pi}{\sqrt{\det(M)}} = \frac{\pi}{\sqrt{\det(\frac{1}{2}\Sigma^{-1})}} = \frac{\pi}{\sqrt{\frac{1}{2^2} \det(\Sigma^{-1})}} = 2\pi \sqrt{\det(\Sigma)}$$

$$\boxed{\therefore \frac{1}{Z} = \frac{1}{2\pi \sqrt{\det(\Sigma)}}} \tag{22}$$

Putting everything together, the bivariate density when the mean is $[0, 0]^T$ is:

$$p(\mathbf{X}) = \frac{1}{Z} e^{-\mathbf{x}^T \mathbf{M} \mathbf{x}} = \frac{1}{2\pi \sqrt{\det(\Sigma)}} e^{-\frac{1}{2} \mathbf{x}^T \Sigma^{-1} \mathbf{x}} \tag{23}$$

If we had started with an ellipse with center $\mu = [\mu_1, \mu_2]^T$, then the density would be:

$$\boxed{p(\mathbf{x}) = \frac{1}{2\pi \sqrt{\det(\Sigma)}} e^{-\frac{1}{2} (\mathbf{x} - \mu)^T \Sigma^{-1} (\mathbf{x} - \mu)}} \tag{24}$$

This can be generalized to n -dimensional normal distribution as:

$$p(\mathbf{x}) = \frac{1}{(2\pi)^{n/2} \sqrt{\det(\Sigma)}} e^{-\frac{1}{2}(\mathbf{x}-\mu)^T \Sigma^{-1}(\mathbf{x}-\mu)} \quad (25)$$

2 Bivariate normal and regression

We can write the Eq(24) in an algebraic form:

$$p(x_1, x_2) = \frac{1}{2\pi\sqrt{\det \Sigma}} \exp\left(-\frac{1}{2}(\mathbf{x}-\mu)^T \Sigma^{-1}(\mathbf{x}-\mu)\right) \quad (26)$$

where,

$$(\mathbf{x}-\mu)^T \Sigma^{-1}(\mathbf{x}-\mu) = \frac{1}{1-r^2} \left[\frac{(x_1-\mu_1)^2}{\sigma_{x_1}^2} - 2r \frac{(x_1-\mu_1)(x_2-\mu_2)}{\sigma_{x_1}\sigma_{x_2}} + \frac{(x_2-\mu_2)^2}{\sigma_{x_2}^2} \right] \quad (27)$$

where r is the correlation coefficient of x_1 and x_2 . Let us look at the conditional distribution of X_2 given X_1 . To do this, let us not worry about the normalization constant, and any terms that depend only on X_1 as we are fixing that. Thus:

$$X_2|X_1 \sim K \exp\left(\frac{-1}{2(1-r^2)\sigma_{x_2}^2} \left[(x_2-\mu_2)^2 - 2r \frac{\sigma_{x_2}}{\sigma_{x_1}} (x_1-\mu_1)(x_2-\mu_2) \right] \right) \quad (28)$$

where K does not depend on x_2 . Completing the squares in $(x_2-\mu_2)$, we get:

$$X_2|X_1 \sim K \exp\left(\frac{-1}{2(1-r^2)\sigma_{x_2}^2} \left[(x_2-\mu_2) - r \frac{\sigma_{x_2}}{\sigma_{x_1}} (x_1-\mu_1) \right]^2 + \frac{r^2}{2(1-r^2)\sigma_{x_1}^2} (x_1-\mu_1)^2 \right) \quad (29)$$

The factor in the exponential (the last term) that depends on x_1 can be absorbed in K , and then rearranging the remaining factors,

$$X_2|X_1 \sim K \exp\left(\frac{-1}{2(1-r^2)\sigma_{x_2}^2} \left[x_2 - \left(\mu_2 - r \frac{\sigma_{x_2}}{\sigma_{x_1}} \mu_1 + r \frac{\sigma_{x_2}}{\sigma_{x_1}} x_1 \right) \right]^2 \right) \quad (30)$$

But earlier when we considered the linear regression model $X_2 = \beta_0 + \beta_1 X_1 + \eta$ where $\eta \sim \mathcal{N}(0, \sigma^2)$, we had proved that:

$$\begin{aligned} \beta_1 &= r \frac{\sigma_{x_2}}{\sigma_{x_1}} \\ \beta_0 &= \mu_2 - \beta_1 \mu_1 = \mu_2 - r \frac{\sigma_{x_2}}{\sigma_{x_1}} \mu_1 \end{aligned} \quad (31)$$

Thus, we see that the conditional distribution of X_2 given X_1 is just Gaussian with $\mathbb{E}(X_2|X_1)$ varying linearly with $\mathbb{E}(X_1)$! This implies that when the joint density of (X_1, X_2) is bivariate Gaussian, the relationship between them is forced to be linear, and any other complex models (for example, quadratic) of the relationship cannot be used.